formatting

theories/models/delayexcept_model.v
@@ -1,7 +1,13 @@
+(* monae: Monadic equational reasoning in Coq                                 *)
+(* Copyright (C) 2025 monae authors, license: LGPL-2.1-or-later               *)
 From mathcomp Require Import all_ssreflect.
 From mathcomp Require boolp.
 From HB Require Import structures.
 Require Import monad_transformer hierarchy.
+
+(**md**************************************************************************)
+(* # Combination of the Delay monad with the exception monad transformer      *)
+(******************************************************************************)
 
 Set Implicit Arguments.
 Unset Strict Implicit.
@@ -13,6 +19,7 @@ Module exceptTdelay.
 Section exceptTdelay.
 Variable M : delayMonad.
 Notation DE := (MX unit M).
+
 Definition DEA {A B} : DE (A + B) -> M ((unit + A) + B )%type :=
   M # (fun uab => match uab with
                  | inl u => inl (inl u)
@@ -21,23 +28,37 @@ Definition DEA {A B} : DE (A + B) -> M ((unit + A) + B )%type :=
                             |inr b => inr b
                             end
                  end).
-Definition whileDE {A B} (body : A -> DE (B + A)) (x : A) : DE B := while (DEA \o body) x.
+
+Definition whileDE {A B} (body : A -> DE (B + A)) (x : A) : DE B :=
+  while (DEA \o body) x.
+
 Definition wBisimDE {A} (d1 d2 : DE A) := wBisim d1 d2.
-Lemma wBisimDE_refl A (a : DE A) : wBisimDE a a.
-Proof. by apply wBisim_refl. Qed.
-Lemma wBisimDE_sym A (d1 d2 : DE A) : wBisimDE d1 d2 -> wBisimDE d2 d1.
-Proof. by apply wBisim_sym. Qed.
-Lemma wBisimDE_trans A (d1 d2 d3 : DE A) : wBisimDE d1 d2 -> wBisimDE d2 d3 -> wBisimDE d1 d3.
-Proof. by apply wBisim_trans. Qed.
-Notation "a '≈' b" := (wBisimDE a b).
+
+Local Notation "a '≈' b" := (wBisimDE a b).
+
+Lemma wBisimDE_refl A (a : DE A) : a ≈ a.
+Proof. exact: wBisim_refl. Qed.
+
+Lemma wBisimDE_sym A (d1 d2 : DE A) : d1 ≈ d2 -> d2 ≈ d1.
+Proof. exact: wBisim_sym. Qed.
+
+Lemma wBisimDE_trans A (d1 d2 d3 : DE A) :
+  d1 ≈ d2 -> d2 ≈ d3 -> d1 ≈ d3.
+Proof. exact: wBisim_trans. Qed.
+
 Hint Extern 0 (wBisimDE _ _) => setoid_reflexivity.
 Hint Extern 0 (wBisim _ _) => setoid_reflexivity.
-Lemma bindXE {A B} (f : A -> DE B) (d : DE A): d >>= f = (@bind M _ _ d (fun (c : unit + A) => match c with |inl z => Ret (inl z) | inr x => f x end)).
+
+Lemma bindXE {A B} (f : A -> DE B) (d : DE A) :
+  d >>= f = (@bind M _ _ d (fun (c : unit + A) => match c with inl z => Ret (inl z) | inr x => f x end)).
 Proof. by rewrite{1}/bind/=/bindX. Qed.
-Lemma bindmwBDE {A B} (f : A -> DE B) (d1 d2 : DE A) : d1 ≈ d2 -> d1 >>= f ≈ d2 >>= f.
-Proof.
-by move => Hd12; rewrite bindXE (bindmwB _ _ _ _ _ Hd12). Qed.
-Lemma bindfwBDE {A B} (f g : A -> DE B) (d : DE A) : (forall a, f a ≈ g a) -> d >>= f ≈ d >>= g.
+
+Lemma bindmwBDE {A B} (f : A -> DE B) (d1 d2 : DE A) :
+  d1 ≈ d2 -> d1 >>= f ≈ d2 >>= f.
+Proof. by move => Hd12; rewrite bindXE (bindmwB _ _ _ _ _ Hd12). Qed.
+
+Lemma bindfwBDE {A B} (f g : A -> DE B) (d : DE A) :
+  (forall a, f a ≈ g a) -> d >>= f ≈ d >>= g.
 Proof.
 move => H.
 rewrite! bindXE.
@@ -45,25 +66,28 @@ set f' := fun c => _.
 set g' := fun c => _.
 rewrite (bindfwB _ _ f' g') // => a.
 subst f' g'.
-by case: a => //=.
+by case: a.
 Qed.
-Lemma fixpointDEE {A B} (f : A -> DE (B + A)) :
-  forall (a : A), whileDE f a ≈ (f a) >>= (sum_rect (fun => DE B ) (@ret DE B ) (whileDE f)).
+
+Lemma fixpointDEE {A B} (f : A -> DE (B + A)) (a : A) :
+  whileDE f a ≈ f a >>= sum_rect (fun => DE B ) (@ret DE B ) (whileDE f).
 Proof.
-move => a.
-rewrite/whileDE/DEA fixpointE /= fmapE /= bindA.
+rewrite /whileDE /DEA fixpointE /= fmapE /= bindA.
 apply (bindfwB _ _ _ _ (f a)) => uba.
-case: uba => [u|[b'|a']] /=; by rewrite bindretf.
+by case: uba => [u|[b'|a']] /=; rewrite bindretf.
 Qed.
+
 Lemma naturalityDEE {A B C} (f : A -> DE (B + A)) (g : B -> DE C) (a : A) :
-@bind DE _ _  (whileDE f a) g ≈
-  whileDE (fun y => (f y) >>= (sum_rect (fun => DE (C + A)) (DE # inl \o g) (DE # inr \o (@ret DE A )))) a.
+  whileDE f a >>= g ≈
+  whileDE (fun y => f y >>= sum_rect (fun => DE (C + A))
+                                     (DE # inl \o g)
+                                     (DE # inr \o (@ret DE A))) a.
 Proof.
-rewrite/whileDE/DEA bindXE naturalityE.
+rewrite /whileDE /DEA bindXE naturalityE.
 apply: whilewB => a' /=.
 rewrite fmapE fmapE !bindA.
-apply: (bindfwB _ _ _ _ (f a')) => uba.
-case: uba => [u|[b''|a'']] /=.
+apply: (bindfwB _ _ _ _ (f a')).
+move=> [u|[b''|a'']] /=.
 - by rewrite !bindretf /= fmapE bindretf.
 - rewrite !bindretf /= fmapE /= fmapE bindA.
   by apply: bindfwB => -[u|c]; rewrite bindretf.
@@ -75,13 +99,13 @@ Lemma codiagonalDEE {A B} (f : A -> DE ((B + A) + A)) (a : A) :
   ≈
   whileDE (whileDE f) a.
 Proof.
-rewrite/whileDE/DEA/=.
+rewrite /whileDE /DEA/=.
 set g := {2} (fun uab => _).
 setoid_symmetry.
 apply: wBisim_trans.
   apply whilewB => a' /=.
   set m := {1}(while _ ).
-  by rewrite (fmapE g (m a')) naturalityE //.
+  by rewrite (fmapE g (m a')) naturalityE.
 rewrite -codiagonalE.
 apply whilewB => a' /=.
 rewrite !fmapE !bindA.
@@ -101,8 +125,11 @@ exact: Hfg.
 Qed.
 
 Lemma uniformDEE {A B C} (f : A -> DE (B + A)) (g : C -> DE (B + C)) (h : C -> A) :
-  (forall c, (f (h c) = (g c >>= sum_rect (fun => DE (B + A)) ((DE # inl) \o Ret) ((DE # inr) \o Ret \o h)))) ->
-  forall c, (whileDE f) (h c) ≈ whileDE g c.
+  (forall c, f (h c) =
+             (g c >>= sum_rect (fun => DE (B + A))
+                               ((DE # inl) \o Ret)
+                               ((DE # inr) \o Ret \o h))) ->
+  forall c, whileDE f (h c) ≈ whileDE g c.
 Proof.
 move=> H c.
 rewrite /whileDE.
